thy/Examples/Synology_Diskstation_DS414/Analyze_Synology_Diskstation.thy
@@ -309,7 +309,9 @@ lemma "check_simple_fw_preconditions (upper_closure (optimize_matches abstract_f
 
 value[code] "map simple_rule_toString (to_simple_firewall
               (upper_closure (optimize_matches abstract_for_simple_firewall (upper_closure (packet_assume_new (unfold_ruleset_INPUT ds2015_fw_INPUT_default_policy (map_of ds2015_fw)))))))"
-
-
+lemma "simple_firewall_valid (to_simple_firewall
+              (upper_closure (optimize_matches abstract_for_simple_firewall (upper_closure (packet_assume_new (unfold_ruleset_INPUT ds2015_fw_INPUT_default_policy (map_of ds2015_fw)))))))" by eval
+lemma "simple_firewall_valid (to_simple_firewall
+              (lower_closure (optimize_matches abstract_for_simple_firewall (upper_closure (packet_assume_new (unfold_ruleset_INPUT ds2015_fw_INPUT_default_policy (map_of ds2015_fw)))))))" by eval
 
 end
